simulations/ctxrefine/CtxRefine.v
@@ -8,8 +8,8 @@ Require Import ModSim.
 Section REFINE.
 
   Definition refines_modsem (ms_src ms_tgt: ModSem.t): Prop :=
-    Beh.of_program (ModSem.compile ms_tgt) <1=
-    Beh.of_program (ModSem.compile ms_src)
+    Beh.of_itree (ModSem.compile ms_tgt) <1=
+    Beh.of_itree (ModSem.compile ms_src)
   .
 
 End REFINE.
